Add another fusion to adc-fusion
Might have something to do with #213.

Also, RewriteAddToAdcInterp is now a bit more stable under changes to
the rewriting strategy (the parts are now more separate).

src/Compilers/Z/Named/RewriteAddToAdc.v
@@ -41,36 +41,86 @@ Section named.
                 (List.fold_left orb (List.map (name_beq n) ns) false)
        end.
 
-  Definition do_rewrite
-             {t} (e : exprf t)
-    : option (exprf t)
-    := match e in Named.exprf _ _ _ t return option (exprf t) with
-       |           (nlet (a2, c1) : tZ * tZ := (ADD bw1 a b as ex0) in P0)
-         => match P0 in Named.exprf _ _ _ t return option (exprf t) with
-            |      (nlet (s , c2) : tZ * tZ := (ADD bw2 c0 (Var _ a2') as ex1) in P1)
-              => match P1 in Named.exprf _ _ _ t return option (exprf t) with
-                 | (nlet c        : tZ      := (ADX (Var _ c1') (Var _ c2') as ex2) in P)
-                   => if (((bw1 =Z? bw2) && (a2 =n? a2') && (c1 =n? c1') && (c2 =n? c2'))
-                            && (is_const_or_var c0 && is_const_or_var a && is_const_or_var b)
-                            && negb (name_list_has_duplicate (a2::c1::s::c2::c::nil ++ get_namesf c0 ++ get_namesf a ++ get_namesf b)%list))
-                      then Some (nlet (a2, c1) : tZ * tZ := ex0 in
-                                 nlet (s , c2) : tZ * tZ := ex1 in
-                                 nlet c        : tZ      := ex2 in
-                                 nlet (s, c)   : tZ * tZ := ADC bw1 c0 a b in
-                                 P)
-                      else None
-                 | P1' => None
-                 end
-            | P0' => None
-            end
+  Definition invertT t
+    := option ((Name * Name * Z * exprf tZ * exprf tZ)
+               * (Name * Name * Z * exprf tZ * Name)
+               * (((Name * Name * Name) * exprf t)
+                  + exprf t)).
+
+  Definition invert_for_do_rewrite_step1 {t} (e : exprf t)
+    : option ((Name * Name * Z * exprf tZ * exprf tZ) * exprf t)
+    := match e in Named.exprf _ _ _ t return option ((Name * Name * Z * exprf tZ * exprf tZ) * exprf t) with
+       | (nlet (a2, c1) : tZ * tZ := (ADD bw1 a b as ex0) in P0)
+         => Some ((a2, c1, bw1, a, b), P0)
+       | _ => None
+       end%core%nexpr%bool.
+  Definition invert_for_do_rewrite_step2 {t} (e : exprf t)
+    : option ((Name * Name * Z * exprf tZ * Name) * exprf t)
+    := match e in Named.exprf _ _ _ t return option ((Name * Name * Z * exprf tZ * Name) * exprf t) with
+       | (nlet (s , c2) : tZ * tZ := (ADD bw2 c0 (Var TZ a2') as ex1) in P1)
+         => Some ((s, c2, bw2, c0, a2'), P1)
+       | _ => None
+       end%core%nexpr%bool.
+  Definition invert_for_do_rewrite_step3 {t} (e : exprf t)
+    : option ((Name * Name * Name) * exprf t)
+    := match e in Named.exprf _ _ _ t return option ((Name * Name * Name) * exprf t) with
+       | (nlet c        : tZ      := (ADX (Var TZ c1') (Var TZ c2') as ex2) in P)
+         => Some ((c, c1', c2'), P)
        | _ => None
        end%core%nexpr%bool.
 
-  Definition do_rewriteo {t} (e : exprf t) : exprf t
-    := match do_rewrite e with
-       | Some e' => e'
-       | None => e
-       end.
+  Definition invert_for_do_rewrite {t} (e : exprf t)
+    : invertT t
+    := match invert_for_do_rewrite_step1 e with
+       | Some ((a2, c1, bw1, a, b), P0)          (* (nlet (a2, c1) : tZ * tZ := (ADD bw1 a b as ex0) in P0) *)
+         => match invert_for_do_rewrite_step2 P0 with
+            | Some ((s, c2, bw2, c0, a2'), P1)   (* (nlet (s , c2) : tZ * tZ := (ADD bw2 c0 (Var TZ a2') as ex1) in P1) *)
+              => match match invert_for_do_rewrite_step3 P1 with
+                       | Some ((c, c1', c2'), P) (* (nlet c        : tZ      := (ADX (Var TZ c1') (Var TZ c2') as ex2) in P) as P1' *)
+                         => if (((bw1 =Z? bw2) && (a2 =n? a2') && (c1 =n? c1') && (c2 =n? c2'))
+                                  && (is_const_or_var c0 && is_const_or_var a && is_const_or_var b)
+                                  && negb (name_list_has_duplicate (a2::c1::s::c2::c::nil ++ get_namesf c0 ++ get_namesf a ++ get_namesf b)%list))
+                            then Some ((a2, c1, bw1, a, b),
+                                       (s, c2, bw2, c0, a2'),
+                                       inl ((c, c1', c2'), P))
+                            else None
+                       | None => None
+                       end with
+                 | Some v => Some v
+                 | None => if (((bw1 =Z? bw2) && (a2 =n? a2'))
+                                 && (is_const_or_var c0 && is_const_or_var a && is_const_or_var b)
+                                 && negb (name_list_has_duplicate (a2::c1::s::c2::nil ++ get_namesf c0 ++ get_namesf a ++ get_namesf b)%list))
+                           then Some ((a2, c1, bw1, a, b),
+                                      (s, c2, bw2, c0, a2'),
+                                      inr P1)
+                           else None
+                 end
+            | None => None
+            end
+       | None => None
+       end%core%nexpr%bool.
+
+  Definition do_rewrite {t} (e : exprf t)
+    : exprf t
+    := match invert_for_do_rewrite e with
+       | Some ((a2, c1, bw1, a, b),
+               (s, c2, bw2, c0, a2'),
+               inl ((c, c1', c2'), P))
+         => (nlet (a2, c1) : tZ * tZ := ADD bw1 a b in
+             nlet (s , c2) : tZ * tZ := ADD bw2 c0 (Var a2') in
+             nlet c        : tZ      := ADX (Var c1') (Var c2') in
+             nlet (s, c)   : tZ * tZ := ADC bw1 c0 a b in
+             P)
+       | Some ((a2, c1, bw1, a, b),
+               (s, c2, bw2, c0, a2'),
+               inr P)
+         => (nlet (a2, c1) : tZ * tZ := ADD bw1 a b in
+             nlet (s , c2) : tZ * tZ := ADD bw2 c0 (Var a2') in
+             nlet s        : tZ      := (nlet (s, c1) : tZ * tZ := ADC bw1 c0 a b in Var s) in
+             P)
+       | None
+         => e
+       end%core%nexpr.
 
   Definition rewrite_exprf_prestep
              (rewrite_exprf : forall {t} (e : exprf t), exprf t)
@@ -88,7 +138,7 @@ Section named.
        end%nexpr.
 
   Fixpoint rewrite_exprf {t} (e : exprf t) : exprf t
-    := do_rewriteo (@rewrite_exprf_prestep (@rewrite_exprf) t e).
+    := do_rewrite (@rewrite_exprf_prestep (@rewrite_exprf) t e).
 
   Definition rewrite_expr {t} (e : expr t) : expr t
     := match e in Named.expr _ _ _ t return expr t with
