src/Compilers/Z/Named/RewriteAddToAdcInterp.v
@@ -6,15 +6,18 @@ Require Import Crypto.Compilers.Syntax.
 Require Import Crypto.Compilers.Z.Syntax.
 Require Import Crypto.Compilers.Z.Syntax.Equality.
 Require Import Crypto.Compilers.Z.Named.RewriteAddToAdc.
+Require Import Crypto.Compilers.Named.GetNames.
 Require Import Crypto.Compilers.Named.Syntax.
 Require Import Crypto.Util.Notations.
 Require Import Crypto.Util.Option.
+Require Import Crypto.Util.Sum.
 Require Import Crypto.Util.Tactics.DestructHead.
 Require Import Crypto.Util.Tactics.BreakMatch.
 Require Import Crypto.Util.Prod.
 Require Import Crypto.Util.LetIn.
 Require Import Crypto.Util.Bool.
 Require Import Crypto.Util.ZUtil.AddGetCarry.
+Require Import Crypto.Util.ListUtil.FoldBool.
 Require Import Crypto.Util.Decidable.
 
 Local Open Scope Z_scope.
@@ -27,10 +30,11 @@ Section named.
           (Name_bl : forall n1 n2, Name_beq n1 n2 = true -> n1 = n2)
           (Name_lb : forall n1 n2, n1 = n2 -> Name_beq n1 n2 = true).
 
+  Local Notation name_list_has_duplicate := (@name_list_has_duplicate Name Name_beq).
   Local Notation exprf := (@exprf base_type op Name).
   Local Notation expr := (@expr base_type op Name).
   Local Notation do_rewrite := (@do_rewrite Name Name_beq).
-  Local Notation do_rewriteo := (@do_rewriteo Name Name_beq).
+  Local Notation invert_for_do_rewrite := (@invert_for_do_rewrite Name Name_beq).
   Local Notation rewrite_exprf := (@rewrite_exprf Name Name_beq).
   Local Notation rewrite_exprf_prestep := (@rewrite_exprf_prestep Name).
   Local Notation rewrite_expr := (@rewrite_expr Name Name_beq).
@@ -49,13 +53,16 @@ Section named.
                                      (Pair (Pair (t1:=tZ) c (t2:=tZ) x) (t2:=tZ) y)).
   Local Notation ADD bw x y := (ADC bw (Op (OpConst 0) TT) x y).
   Local Notation ADX x y := (Op (@Add TZ TZ TZ) (Pair (t1:=tZ) x (t2:=tZ) y)).
+  Local Infix "=Z?" := Z.eqb.
+  Local Infix "=n?" := Name_beq.
 
   Local Ltac simple_t_step :=
-    first [ discriminate
-          | exact I
+    first [ exact I
           | progress intros
           | progress subst
-          | progress inversion_option ].
+          | progress inversion_option
+          | progress inversion_sum
+          | progress inversion_prod ].
   Local Ltac destruct_t_step :=
     first [ break_innermost_match_hyps_step
           | break_innermost_match_step ].
@@ -91,17 +98,77 @@ Section named.
                  end ];
          try exact I
     end.
-  Local Ltac small_inversion_step _ :=
+  Local Ltac small_inversion_prestep _ :=
     match goal with
     | [ H : match ?e with _ => _ end = Some _ |- _ ] => do_small_inversion e
     | [ H : match ?e with _ => _ end = true |- _ ] => do_small_inversion e
     | [ H : match ?e with _ => _ end _ = Some _ |- _ ] => do_small_inversion e
     end.
+  Local Ltac small_inversion_step :=
+    small_inversion_prestep (); break_innermost_match; intros; try exact I.
 
+  Local Ltac t_rewrite_step_correct_step :=
+    first [ reflexivity
+          | progress inversion_option
+          | simple_t_step
+          | break_innermost_match_hyps_step
+          | small_inversion_step
+          | progress unfold invert_for_do_rewrite_step1, invert_for_do_rewrite_step2, invert_for_do_rewrite_step3 in * ].
+  Local Ltac t_rewrite_step_correct := repeat t_rewrite_step_correct_step.
+
+  Local Ltac mk_lookupb_extendb_lemma_debug := constr:(false).
+  Local Ltac debug_print_fail tac :=
+    let lvl := mk_lookupb_extendb_lemma_debug in
+    lazymatch lvl with
+    | true => let dummy := match goal with
+                           | _ => tac ()
+                           end in
+              constr:(I : I)
+    | false => constr:(I : I)
+    | _ => let TRUE := uconstr:(true) in
+           let FALSE := uconstr:(false) in
+           let dummy := match goal with
+                        | _ => idtac "Error: Invalid mk_lookupb_extendb_lemma_debug level" lvl "which is neither" TRUE "nor" FALSE
+                        end in
+           constr:(I : I)
+    end.
+
+  (** We build the lemma explicitly, because letting [rewrite] and
+     [assumption || congruence] pick out the hypotheses and build the
+     lemmas is actually a bottleneck (timesavings: about 25s) *)
+  Local Ltac mk_lookupb_extendb_lemma base_type_code Name var Context t t' ctx n n' v :=
+    lazymatch n with
+    | n' => lazymatch t with
+            | t' => constr:(@lookupb_extendb_same base_type_code Name var Context _ ctx n t v)
+            | _ => let lem := constr:(@lookupb_extendb_wrong_type base_type_code Name var Context _ ctx n t t' v) in
+                   lazymatch goal with
+                   | [ H : t <> t' |- _ ]
+                     => constr:(lem H)
+                   | [ H : t' <> t |- _ ]
+                     => constr:(lem (@not_eq_sym _ _ _ H))
+                   | _ => let HT := uconstr:(t <> t') in
+                          debug_print_fail ltac:(fun _ => idtac "Error in mk_lookupb_exntedb_lemma: could not find hypothesis of type" HT)
+                   end
+            end
+    | _ => let lem := constr:(@lookupb_extendb_different base_type_code Name var Context _ ctx n n' t t' v) in
+           lazymatch goal with
+           | [ H : n <> n' |- _ ]
+             => constr:(lem H)
+           | [ H : n' <> n |- _ ]
+             => constr:(lem (@not_eq_sym _ _ _ H))
+           | _ => let HT := uconstr:(n <> n') in
+                  debug_print_fail ltac:(fun _ => idtac "Error in mk_lookupb_exntedb_lemma: could not find hypothesis of type" HT)
+           end
+    end.
   Local Ltac rewrite_lookupb_step :=
-    first [ rewrite !lookupb_extendb_different in * by (assumption || congruence)
-          | rewrite !lookupb_extendb_same in * by assumption
-          | rewrite !lookupb_extendb_wrong_type in * by (assumption || congruence)
+    first [ match goal with
+            | [ H : context[@lookupb ?base_type_code ?Name ?var ?Context ?t' (extendb (t:=?t) ?ctx ?n ?v) ?n'] |- _ ]
+              => let lem := mk_lookupb_extendb_lemma base_type_code Name var Context t t' ctx n n' v in
+                 rewrite lem in H
+            | [ |- context[@lookupb ?base_type_code ?Name ?var ?Context ?t' (extendb (t:=?t) ?ctx ?n ?v) ?n'] ]
+              => let lem := mk_lookupb_extendb_lemma base_type_code Name var Context t t' ctx n n' v in
+                 rewrite lem
+            end
           | match goal with
             | [ H : context[lookupb (extendb _ _ _) _] |- _ ] => revert H
             | [ |- context[lookupb (extendb _ ?n _) ?n'] ]
@@ -134,78 +201,187 @@ Section named.
   Local Ltac do_rewrite_adc :=
     first [ do_rewrite_adc' uconstr:(fun a b => Some b)
           | do_rewrite_adc' uconstr:(fun a b => Some a) ].
+  Local Ltac do_small_inversion_ctx :=
+    repeat match goal with
+           | [ H : is_const_or_var ?e = true |- _ ]
+             => do_small_inversion e; break_innermost_match; intros; try exact I;
+                simpl in H; try solve [ clear -H; discriminate ]
+           | [ H : match ?e with _ => _ end = true |- _ ]
+             => do_small_inversion e; break_innermost_match; intros; try exact I;
+                simpl in H; try solve [ clear -H; discriminate ]
+           | [ H : match ?e with _ => _ end _ = true |- _ ]
+             => do_small_inversion e; break_innermost_match; intros; try exact I;
+                simpl in H; try solve [ clear -H; discriminate ]
+           end.
+  Local Ltac t_fin_step :=
+    match goal with
+    | [ |- ?x = ?x ] => reflexivity
+    | [ H : ?x = Some _ |- context[?x] ] => rewrite H
+    | [ H : ?x = None |- context[?x] ] => rewrite H
+    | [ H : ?x = Some ?a, H' : ?x = Some ?b |- _ ]
+      => assert (a = b) by congruence; (subst a || subst b)
+    | [ H : interpf ?x = Some ?v, H' : interpf ?x = None |- interpf _ = None ]
+      => cut (Some v = None);
+         [ congruence | rewrite <- H, <- H'; clear H H' ]
+    | _ => progress rewrite_lookupb
+    | _ => progress simpl in *
+    | _ => progress intros
+    | _ => progress subst
+    | _ => progress inversion_option
+    | [ |- (dlet x := _ in _) = (dlet y := _ in _) ]
+      => apply Proper_Let_In_nd_changebody_eq; intros ??
+    | _ => progress unfold Let_In
+    | [ |- interpf ?x = interpf ?x ]
+      => eapply @interpf_Proper; [ eauto with typeclass_instances.. | intros ?? | reflexivity ]
+    | _ => progress break_innermost_match; try reflexivity
+    | _ => progress break_innermost_match_hyps; try reflexivity
+    | _ => progress break_match; try reflexivity
+    end.
+  Local Ltac t_fin :=
+    repeat t_fin_step;
+    try do_rewrite_adc.
+
+
+  Lemma invert_for_do_rewrite_step1_correct {t} {e : exprf t} {v}
+        (H : invert_for_do_rewrite_step1 e = Some v)
+    : e = let '((a2, c1, bw1, a, b), P) := v in
+          (nlet (a2, c1) : tZ * tZ := ADD bw1 a b in P)%nexpr.
+  Proof. t_rewrite_step_correct. Qed.
+  Lemma invert_for_do_rewrite_step2_correct {t} {e : exprf t} {v}
+        (H : invert_for_do_rewrite_step2 e = Some v)
+    : e = let '((s, c2, bw2, c0, a2'), P) := v in
+          (nlet (s , c2) : tZ * tZ := (ADD bw2 c0 (Var a2')) in P)%nexpr.
+  Proof. t_rewrite_step_correct. Qed.
+  Lemma invert_for_do_rewrite_step3_correct {t} {e : exprf t} {v}
+        (H : invert_for_do_rewrite_step3 e = Some v)
+    : e = let '((c, c1', c2'), P) := v in
+          (nlet c        : tZ      := (ADX (Var c1') (Var c2')) in P)%nexpr.
+  Proof. t_rewrite_step_correct. Qed.
+
+  Lemma invert_for_do_rewrite_correct {t} {e : exprf t} {v}
+        (H : invert_for_do_rewrite e = Some v)
+    : match v with
+      | ((a2, c1, bw1, a, b),
+         (s, c2, bw2, c0, a2'),
+         inl ((c, c1', c2'), P))
+        => (nlet (a2, c1) : tZ * tZ := ADD bw1 a b in
+            nlet (s , c2) : tZ * tZ := ADD bw2 c0 (Var a2') in
+            nlet c        : tZ      := ADX (Var c1') (Var c2') in
+            P) = e
+           /\ ((((bw1 =Z? bw2) && (a2 =n? a2') && (c1 =n? c1') && (c2 =n? c2'))
+                  && (is_const_or_var c0 && is_const_or_var a && is_const_or_var b)
+                  && negb (name_list_has_duplicate (a2::c1::s::c2::c::nil ++ get_namesf c0 ++ get_namesf a ++ get_namesf b)%list))
+               = true)
+      | ((a2, c1, bw1, a, b),
+         (s, c2, bw2, c0, a2'),
+         inr P)
+        => (nlet (a2, c1) : tZ * tZ := ADD bw1 a b in
+            nlet (s , c2) : tZ * tZ := ADD bw2 c0 (Var a2') in
+            P) = e
+           /\ ((((bw1 =Z? bw2) && (a2 =n? a2'))
+                  && (is_const_or_var c0 && is_const_or_var a && is_const_or_var b)
+                  && negb (name_list_has_duplicate (a2::c1::s::c2::nil ++ get_namesf c0 ++ get_namesf a ++ get_namesf b)%list))
+               = true)
+      end%core%nexpr%bool.
+  Proof.
+    unfold invert_for_do_rewrite in H; break_innermost_match_hyps;
+      repeat first [ progress subst
+                   | progress inversion_option
+                   | progress inversion_sum
+                   | progress inversion_prod
+                   | match goal with
+                     | [ H : _ = Some _ |- _ ]
+                       => first [ rewrite (invert_for_do_rewrite_step1_correct H)
+                                | rewrite (invert_for_do_rewrite_step2_correct H)
+                                | rewrite (invert_for_do_rewrite_step3_correct H) ]
+                     | [ H : ?x = true |- _ ] => rewrite H; clear H
+                     | [ |- _ /\ _ ] => split
+                     | [ |- ?x = ?x ] => reflexivity
+                     | [ H : Name_beq _ _ = true |- _ ] => apply Name_bl in H
+                     | [ H : Z.eqb _ _ = true |- _ ] => apply Z.eqb_eq in H
+                     | [ H : Name_beq ?x ?y = false |- _ ]
+                       => assert (x <> y) by (clear -H Name_lb; intro; rewrite Name_lb in H by assumption; congruence);
+                          clear H
+                     end
+                   | progress rewrite !Bool.negb_orb in *
+                   | progress rewrite !Bool.negb_true_iff in *
+                   | progress split_andb
+                   | progress simpl @negb in *
+                   | progress do_small_inversion_ctx ].
+  Qed.
 
   Lemma interpf_do_rewrite
-        {t} {e e' : exprf t}
-        (H : do_rewrite e = Some e')
-    : retT e e'.
+        {t} {e : exprf t}
+    : retT e (do_rewrite e).
   Proof.
-    unfold do_rewrite in H;
-      repeat first [ simple_t_step
-                   | small_inversion_step ()
-                   | destruct_t_step ].
-    Time all:match goal with
-             | [ H : _ = ?x |- _ = ?x ] => rewrite <- H; clear H
-             end.
-    Time all:split_andb.
-    Time all:progress simpl @negb in *.
-    Time all:repeat match goal with
-                    | [ H : Name_beq _ _ = true |- _ ] => apply Name_bl in H
-                    | [ H : Z.eqb _ _ = true |- _ ] => apply Z.eqb_eq in H
-                    end.
-    Time all:subst.
-    Local Ltac do_small_inversion_ctx :=
-      repeat match goal with
-             | [ H : is_const_or_var ?e = true |- _ ]
-               => do_small_inversion e; break_innermost_match; intros; try exact I;
-                  simpl in H; try solve [ clear -H; discriminate ]
-             | [ H : match ?e with _ => _ end = true |- _ ]
-               => do_small_inversion e; break_innermost_match; intros; try exact I;
-                  simpl in H; try solve [ clear -H; discriminate ]
-             | [ H : match ?e with _ => _ end _ = true |- _ ]
-               => do_small_inversion e; break_innermost_match; intros; try exact I;
-                  simpl in H; try solve [ clear -H; discriminate ]
-             end.
-    Time all:do_small_inversion_ctx.
-    Time all:simpl @negb in *.
-    Time all:rewrite !Bool.negb_orb in *.
-    Time all:split_andb.
-    Time all:rewrite !Bool.negb_true_iff in *.
-    Time all:repeat
-               match goal with
-               | [ H : Name_beq ?x ?y = false |- _ ]
-                 => assert (x <> y) by (clear -H Name_lb; intro; rewrite Name_lb in H by assumption; congruence);
-                      clear H
-               end.
-    Time all:subst.
-    Time all:simpl @interpf in *.
-    Time all:cbv [interp_op option_map lift_op Zinterp_op] in *; simpl in *.
-    Time all:unfold Let_In in * |- .
-    Time all:break_innermost_match; try reflexivity.
-    Local Ltac t_fin_step :=
-      match goal with
-      | [ |- ?x = ?x ] => reflexivity
-      | [ H : ?x = Some _ |- context[?x] ] => rewrite H
-      | [ H : ?x = None |- context[?x] ] => rewrite H
-      | [ H : ?x = Some ?a, H' : ?x = Some ?b |- _ ]
-        => assert (a = b) by congruence; (subst a || subst b)
-      | _ => progress rewrite_lookupb
-      | _ => progress simpl in *
-      | _ => progress intros
-      | _ => progress subst
-      | _ => progress inversion_option
-      | [ |- (dlet x := _ in _) = (dlet y := _ in _) ]
-        => apply Proper_Let_In_nd_changebody_eq; intros ??
-      | _ => progress unfold Let_In
-      | [ |- interpf ?x = interpf ?x ]
-        => eapply @interpf_Proper; [ eauto with typeclass_instances.. | intros ?? | reflexivity ]
-      | _ => progress break_innermost_match; try reflexivity
-      | _ => progress break_innermost_match_hyps; try reflexivity
-      | _ => progress break_match; try reflexivity
-      end.
-    Local Ltac t_fin :=
-      repeat t_fin_step;
-      try do_rewrite_adc.
+    unfold do_rewrite.
+    pose proof (@invert_for_do_rewrite_correct t e) as H'.
+    break_innermost_match; inversion_option;
+      [ specialize (H' _ eq_refl)
+      | specialize (H' _ eq_refl)
+      | intros; subst; assumption ].
+    all: intros *; let H := fresh in intro H; rewrite <- H; clear H.
+    Time all:repeat first [ progress cbv beta iota in *
+                          | progress destruct_head'_and
+                          | progress subst
+                          | progress rewrite !Bool.negb_orb in *
+                          | progress split_andb
+                          | progress simpl @name_list_has_duplicate in *
+                          | match goal with
+                            | [ H : Name_beq _ _ = true |- _ ] => apply Name_bl in H
+                            | [ H : Z.eqb _ _ = true |- _ ] => apply Z.eqb_eq in H
+                            | [ H : Name_beq ?x ?y = false |- _ ]
+                              => assert (x <> y) by (clear -H Name_lb; intro; rewrite Name_lb in H by assumption; congruence);
+                                   clear H
+                            | [ H : context[List.fold_left orb ?ls ?v] |- _ ]
+                              => lazymatch v with
+                                 | false => fail
+                                 | _ => rewrite (fold_left_orb_pull ls v) in H
+                                 end
+                            end
+                          | progress simpl @List.fold_left in *
+                          | progress do_small_inversion_ctx
+                          | progress rewrite !Bool.negb_true_iff in *
+                          | progress intros *
+                          | match goal with
+                            | [ H : invert_for_do_rewrite _ = Some _ |- _ ] => clear H
+                            end ].
+    Time all: repeat first [ progress simpl
+                           | progress cbv [interp_op option_map lift_op Zinterp_op] in * ].
+    Time all: repeat first [ progress subst
+                           | progress inversion_option
+                           | progress rewrite_lookupb
+                           | progress intros
+                           | match goal with
+                             | [ H : ?x = Some ?a, H' : ?x = Some ?b |- _ ]
+                               => assert (a = b) by congruence; (subst a || subst b)
+                             | [ H : ?T, H' : ?T |- _ ] => clear H'
+                             end ].
+    Set Ltac Profiling.
+    Time all: repeat first [ reflexivity
+                           | progress subst
+                           | progress inversion_option
+                           | progress rewrite_lookupb
+                           | progress intros
+                           | progress cbn [fst snd]
+                           | match goal with
+                             | [ H : ?x = Some ?a, H' : ?x = Some ?b |- _ ]
+                               => assert (a = b) by congruence; (subst a || subst b)
+                             | [ H : ?T, H' : ?T |- _ ] => clear H'
+                             | [ |- context[match lookupb ?ctx ?n with _ => _ end] ]
+                               => is_var ctx; destruct (lookupb ctx n) eqn:?
+                             | [ |- (dlet x := ?e in _) = (dlet y := ?e in _) ]
+                               => apply Proper_Let_In_nd_changebody_eq; intros ??
+                             end
+                           | progress unfold Let_In at 1 ].
+    { Time t_fin. }
+    { Time t_fin. }
+    { Time t_fin. }
+    { Time t_fin. }
+    { Time t_fin. }
+    { Time t_fin. }
+    { Time t_fin. }
+    { Time t_fin. }
     { Time t_fin. }
     { Time t_fin. }
     { Time t_fin. }
@@ -216,15 +392,7 @@ Section named.
     { Time t_fin. }
   Time Qed.
 
-  Lemma interpf_do_rewriteo
-        {t} {e : exprf t}
-    : retT e (do_rewriteo e).
-  Proof.
-    unfold do_rewriteo; intros *; break_innermost_match; try congruence.
-    apply interpf_do_rewrite; assumption.
-  Qed.
-
-  Local Opaque RewriteAddToAdc.do_rewriteo.
+  Local Opaque RewriteAddToAdc.do_rewrite.
   Lemma interpf_rewrite_exprf
         {t} (e : exprf t)
     : retT e (rewrite_exprf e).
@@ -233,7 +401,7 @@ Section named.
     pose (rewrite_exprf_prestep (@rewrite_exprf) e) as E.
     induction e; simpl in *;
       intros ctx v H;
-      pose proof (interpf_do_rewriteo (t:=T) (e:=E) ctx v H); clear H;
+      pose proof (interpf_do_rewrite (t:=T) (e:=E) ctx v H); clear H;
       subst T E;
       repeat first [ assumption
                    | progress unfold option_map, Let_In in *
